\documentclass[12pt]{article}

\begin{document}
$S\ K\ K\ \equiv\ I\ ?\\ $
$S\ \equiv\ \lambda x\ y\ z.x\ z\ (y\ z)\ K\ \equiv\ \lambda x\ y.x\ I\ \equiv\ \lambda x.x\\ $
Proves:\\
$S\ K\ K\ \equiv\ (\lambda x\ y\ z.x\ z\ (y\ z))\ (\lambda x\ y.x)\ (\lambda x\ y.x)\
\equiv\ (\lambda y\ z.(\lambda x\ y.x)\ z\ (y\ z))\ (\lambda x\ y.x) \equiv\\ $
$\equiv\ (\lambda y\ z.(\lambda y.z)\ (y\ z))\ (\lambda x\ y.x) 
\equiv (\lambda y.\lambda z.z)\ (\lambda x\ y.x) \equiv (\lambda z.z) \equiv I\\$
\end{document}